scripts/HolTypeHashes.lean
@@ -58,6 +58,7 @@ import Flapjack.Pancake.Semantics.PanSem.DecExact
 import Flapjack.Pancake.Semantics.PanSem.ReturnRaiseExact
 import Flapjack.Pancake.Semantics.PanSem.EvalExact
 import Flapjack.Pancake.Semantics.PanSem.DecCallExact
+import Flapjack.Pancake.Semantics.PanSem.DeclContextExact
 import Flapjack.Pancake.Semantics.PanSem.EvaluateDeclsExact
 import Flapjack.Pancake.Semantics.PanSem.ClockExact
 import Flapjack.Pancake.Semantics.PanSem.StateSimpExact
